Proposal/main.typ
@@ -115,39 +115,124 @@ Work has already begun defining the semantics of LLVM in Isabelle and creating a
 == LLVM semantics
 
 Part of the LLVM-IR's AST has been defined as datatypes in Isabelle.
-With this part of the AST,  can be passed to  to execute them.
-Such invocations serve as the basis of proofs.
+With this part of the AST, functions made up of instruction blocks can be executed.
 
 The operational semantics are defined as follows:
 - Functions contain multiple labeled instruction blocks and one unlabeled block to be executed first.
-- Instruction blocks have a list of regular instructions to be executed in order and up to one terminator instruction that impacts execution flow.
+- Instruction blocks have a list of regular instructions to be executed in order and one terminator instruction that impacts execution flow.
 - Instructions are executed according to their specification in the LLVM Language Reference Manual.#footnote("https://llvm.org/docs/LangRef.html")
-- Execution state is defined as a triple of registers, a stack, and a heap.
-- The stack and heap use the same underlying memory definition which uses a list of values.
-- The registers use a mapping from a name to a value.
+
+Execution of any single instruction takes in some state and produces a state.
+This state is defined as follows:
+- It is a triple of registers, a stack, and a heap.
+- The stack and heap have the same underlying memory definition: a list of values. They are addressable using indices in these lists.
+- Registers are a mapping from a name to a value. (TODO: change 'registers' to 'SSA-values' in implementation and report)
 
 The regular instructions currently (partly) implemented are:
-- alloca
-- store
-- load
-- icmp
-- add
-- phi
+- alloca - allocates a new address in the stack, and stores the address in some register.
+- store - stores a value at some address in the stack or heap.
+- load - loads a value from some address in the stack or heap into a register.
+- icmp - compares two values (32/64 bit signed/unsigned integers) and stores the result in a register as a single bit (boolean).
+- add - adds two values (32/64 bit signed/unsigned integers) and stores the result in a register (another 32/64 bit integer or a poison value if an overflow occurred).
+- phi - store a value from a list of possible values into a register depending on the instruction block that lead to this block.
 
 The terminator instructions implemented are:
-- br
-- ret
+- br - branch to a different instruction given its label (could always be the same label, or switch based on a boolean value in some register).
+- ret - return from the function with some value.
+
+With this implementation, basic programs consisting of these instructions can already be executed.
+For example, take the following C program:
+```C
+int main() {
+    int y = 1;
+    int x = y?1:0;
+    return x;
+}
+```
+
+This might produce the following LLVM-IR code:
+```llvm
+define dso_local i32 @main() #0 {
+  %1 = alloca i32, align 4
+  %2 = alloca i32, align 4
+  %3 = alloca i32, align 4
+  %4 = alloca i32, align 4
+  store i32 0, ptr %1, align 4
+  store i32 1, ptr %2, align 4
+  %5 = load i32, ptr %2, align 4
+  %6 = icmp ne i32 %5, 0
+  br i1 %6, label %7, label %9
+
+7:
+  store i32 1, ptr %4, align 4
+  %8 = load i32, ptr %4, align 4
+  br label %10
+
+9:
+  br label %10
+
+10:
+  %11 = phi i32 [ %8, %9 ], [ 0, %9 ]
+  store i32 %11, ptr %3, align 4
+  %12 = load i32, ptr %3, align 4
+  ret i32 %12
+}
+```
+
+Encoded into the current AST representation, this becomes:
+```isabelle
+definition pmain :: "llvm_instruction_block" where
+  "pmain = ([
+    alloca ''1'' i32 (Some 4),
+    alloca ''2'' i32 (Some 4),
+    alloca ''3'' i32 (Some 4),
+    alloca ''4'' i32 (Some 4),
+    store i32 (val (vi32 0)) (ptr (reg ''1'')) (Some 4),
+    store i32 (val (vi32 1)) (ptr (reg ''2'')) (Some 4),
+    load ''5'' i32 (ptr (reg ''2'')) (Some 4),
+    icmp ''6'' False comp_ne i32 (reg ''5'') (val (vi32 0))],
+    br_i1 (reg ''6'') ''7'' ''9''
+  )"
+
+definition p7 :: "llvm_instruction_block" where
+  "p7 = ([
+    store i32 (val (vi32 1)) (ptr (reg ''4'')) (Some 4),
+    load ''8'' i32 (ptr (reg ''4'')) (Some 4)],
+    br_label ''10''
+  )"
+
+definition p9 :: "llvm_instruction_block" where
+  "p9 = ([],
+    br_label ''10''
+  )"
+
+definition p10 :: "llvm_instruction_block" where
+  "p10 = ([
+    phi ''11'' i32 [(''7'', reg ''8''), (''9'', val (vi32 0))],
+    store i32 (reg ''11'') (ptr (reg ''3'')) (Some 4),
+    load ''12'' i32 (ptr (reg ''3'')) (Some 4)],
+    ret i32 (reg ''12'')
+  )"
+
+definition phi_main :: "llvm_function" where
+  "phi_main = func (func_def ''main'' i32) pmain [(''7'', p7), (''9'', p9), (''10'', p10)]"
+```
+
+This can be executed as follows, which gives the proper return value:
+```isabelle
+value "execute_function empty_state phi_main"
+```
 
 
 == Weakest precondition mechanics
 
+Taking inspiration from Hoare logic, 
+To reason about the execution of 
 
 
 = Rough planning
 
-- Create abstract register
-- Implement intro rules for registers
-- Implement intro rules at the level of instructions
+- Better LLVM semantics (e.g. register overrides)
 - Support verification condition generation at the level of blocks
 - Add method of specifying pre- and post-conditions for code blocks 
 - Create flowchart view of code blocks
